templates/lockfree/skiplist_v1_traverse.v
@@ -37,6 +37,38 @@ Module SKIPLIST1_SPEC_TRAVERSE.
     (* iAssumption. *)
   Admitted.
 
+  Parameter findNext_spec : ∀ (n: Node) (i: nat),
+     ⊢ (<<< ∀∀ mark next k, node n mark next k >>>
+           findNext #n #i @ ⊤
+       <<< ∃∃ (m: bool) (opt_n': option Node),
+              node n mark next k ∗ ⌜mark !!! i = m⌝ ∗ ⌜next !! i = opt_n'⌝,
+              RET (match opt_n' with None => (#m, NONEV) 
+                                    | Some n' => (#m, SOMEV #n') end) >>>)%I.
+
+  Parameter try_constraint_traverse_spec : ∀ (pred curr new_node: Node) (i: nat),
+     ⊢ (<<< ∀∀ mark next k, node pred mark next k >>>
+           try_constraint #pred #curr #new_node #i @ ⊤
+       <<< ∃∃ (success: bool) next',
+              node pred mark next' k
+            ∗ (match success with true => ⌜next !! i = Some curr 
+                                            ∧ mark !!! i = false
+                                            ∧ next' = <[i := new_node]> next⌝
+                                | false => ⌜(next !! i ≠ Some curr ∨ 
+                                              mark !!! i = true)
+                                            ∧ next' = next⌝ end),
+              RET (match success with true => SOMEV #() 
+                                    | false => NONEV end)  >>>)%I.
+
+  Parameter compareKey_spec : ∀ (n: Node) (k': nat),
+     ⊢ (<<< ∀∀ mark next k, node n mark next k >>>
+           compareKey #n #k' @ ⊤
+       <<< ∃∃ (res: nat),
+              node n mark next k ∗ 
+              ⌜if decide (res = 0) then k < k'
+               else if decide (res = 1) then k = k'
+               else k > k'⌝,
+              RET #res >>>)%I.
+                                    
 
   Definition traversal_inv s i k p c : Prop :=
     p ∈ FP s 
@@ -45,586 +77,415 @@ Module SKIPLIST1_SPEC_TRAVERSE.
   ∧ Marki s p i = false 
   ∧ Nexti s p i = Some c.
 
-(*
-  Lemma traverse_i_spec_high N γ_t γ_s γ_m γ_td γ_ght γ_sy t_id t0 k 
-                           (i: nat) (p c: Node):
-      main_inv N γ_t γ_s γ_m γ_td γ_ght -∗
-        thread_vars γ_t γ_ght γ_sy t_id t0 -∗  
-        {{{ ∃ s, past_state γ_m t0 s ∗ ⌜traversal_inv s i k p c⌝  }}}
-           traverse_i #i #k #p #c
-        {{{ (p' c': Node) (res: bool), 
-              RET (#p', #c', #res);
-              ∃ s, past_state γ_m t0 s ∗ ⌜traversal_inv s i k p' c'⌝ }}}.
+  Lemma traverse_i_spec N γ_t γ_r γ_m γ_td1 γ_td2 γ_ght
+  γ_sy t_id t0 k (i: nat) (p c: Node):
+  main_inv N γ_t γ_r γ_m γ_td1 γ_td2 γ_ght -∗
+    thread_vars γ_t γ_ght γ_sy t_id t0 -∗  
+    {{{ (∃ s, past_state γ_m t0 s ∗ ⌜traversal_inv s i k p c⌝) }}}
+      traverse_i #i #p #c #k
+    {{{ (ores: option (Node * Node * bool)), 
+          RET (match ores with
+                None => NONEV
+              | Some res =>SOMEV (#res.1.1,#res.1.2,#res.2) end);
+          match ores with 
+            None => True
+          | Some res => 
+            let p' := res.1.1 in
+            let c' := res.1.2 in
+            let b := res.2 in
+            (∃ s, past_state γ_m t0 s 
+              ∗ ⌜traversal_inv s i k p' c'⌝
+              ∗ ⌜i = 0 → if b then k ∈ keyset (FI s c') ∧ k = Key s c'
+                          else k ∉ abs s⌝) end }}}.
   Proof.
     iIntros "#HInv #Thd". iLöb as "IH" forall (p c).
     iIntros (Φ) "!# #HtrInv Hpost". wp_lam. wp_pures.
     awp_apply findNext_spec.
     iInv "HInv" as (M0 T0 s0) "(>Ds & >%Habs0 & >Hist & Help & >Templ)".
     { admit. }
-    iDestruct "Templ" as "(Hglob & Res & %PT0 & %Trans_M0)". 
-    set γ_I := skiplist_v1.SKIPLIST1.γ_I.
-    set γ_fp := skiplist_v1.SKIPLIST1.γ_fp.
-    set γ_ks := skiplist_v1.SKIPLIST1.γ_ks.
+    iDestruct "Templ" as "(SShot0 & Res & %PT0 & %Trans_M0)".
+    iDestruct "Res" as "(GKS & Nodes & Nodes_KS)".
     iAssert (⌜c ∈ FP s0⌝)%I as %FP_c0.
     { (* interpolation *) admit. }
     rewrite (big_sepS_delete _ (FP s0) c); last by eauto.
-    iDestruct "Res" as "((Node_c & Node_crest) & Res_rest)".
+    iDestruct "Nodes" as "(Node_c & Nodes_rest)".
     iAaccIntro with "Node_c".
-    { iIntros "Node". iModIntro. iFrame.
+    { iIntros "Node". iModIntro. iFrame "Hpost".
       iNext; iExists M0, T0, s0.
       iFrame "∗%#". 
       rewrite (big_sepS_delete _ (FP s0) c); last by eauto. 
-      iFrame "Res_rest". iFrame. }
+      iFrame "Nodes_rest". iFrame. }
     iIntros (m c') "(Node_c & %Mark_c0 & %Next_c0)".
     iModIntro. iSplitR "Hpost".
-    { iNext. iExists M0, T0, s0.
-      iFrame "∗%".
+    { iNext. iExists M0, T0, s0. iFrame "∗%".
       rewrite (big_sepS_delete _ (FP s0) c); last by eauto.
-      iFrame "Res_rest". iFrame. }
-    clear γ_I γ_fp γ_ks.
-    destruct c' as [c' |]; destruct m; wp_pures. 
+      iFrame "Nodes_rest". iFrame. }
+    destruct c' as [cn |]; destruct m; wp_pures. 
     - awp_apply try_constraint_traverse_spec; try done.
       iInv "HInv" as (M1 T1 s1) "(>Ds & >%Habs1 & >Hist & Help & >Templ)".
       { admit. }
-      iDestruct "Templ" as "(Hglob & Res & %PT1 & %Trans_M1)". 
-      set γ_I := skiplist_v1.SKIPLIST1.γ_I.
-      set γ_fp := skiplist_v1.SKIPLIST1.γ_fp.
-      set γ_ks := skiplist_v1.SKIPLIST1.γ_ks.
+      iDestruct "Templ" as "(SShot1 & Res & %PT1 & %Trans_M1)".
+      iDestruct "Res" as "(GKS & Nodes & Nodes_KS)".
       iAssert (⌜p ∈ FP s1⌝)%I as %FP_p1.
       { (* interpolation *) admit. }
-      iAssert (past_state γ_m t0 s1) as "#Hs1".
-      { admit. }
       rewrite (big_sepS_delete _ (FP s1) p); last by eauto.
-      iDestruct "Res" as "((Node_p & Node_prest) & Res_rest)".
+      iDestruct "Nodes" as "(Node_p & Nodes_rest)".
       iAaccIntro with "Node_p".
-      { iIntros "Node". iModIntro. iFrame.
-        iNext; iExists M1, T1, s1.
-        iFrame "∗%#". 
-        rewrite (big_sepS_delete _ (FP s1) p); last by eauto. 
-        iFrame "Res_rest". iFrame. }
-      iIntros (success next')"(Node_p & Hif)".
+      { iIntros "Node_p". iModIntro. iFrame "Hpost".
+        iNext; iExists M1, T1, s1. iFrame "∗%#". 
+        rewrite (big_sepS_delete _ (FP s1) p); last by eauto. iFrame. }
+      iIntros (success next') "(Node_p & Hsuccess)".
       destruct success.
-      + iDestruct "Hif" as "%H'".
-        destruct H' as [Mark_p1 [Next_p1 Def_next']].
-        iAssert (∃ s, past_state γ_m t0 s ∗ ⌜traversal_inv s i k p c'⌝)%I 
-          as "#HtrInv'".
-        { iExists s1. iFrame "Hs1". iPureIntro.
-          split; try done. admit. admit. }  
+      + iDestruct "Hsuccess" as %[Next_p1 [Mark_p1 Def_next']].
+        destruct (decide (i = 0)) as [-> | Hi0].
+        * iDestruct "SShot1" as %[FP1 [C1 [Mk1 [Nx1 [Ky1 [I1 
+            [Hs1 [Dom_Mk1 [Dom_Nx1 [Dom_Ky1 Dom_I1]]]]]]]]]].
+          set Nx1' := <[p := next']> Nx1.
+          set Ip1 := I1 !!! p. set Ic1 := I1 !!! c. set out_pc := out Ip1 c.
+          set Ip1' := int {| infR := inf_map Ip1; outR :=  <<[cn := out_pc]>> ∅ |}.
+          set Ic1': multiset_flowint_ur nat := 
+            int {| infR := {[c := ∅]}; outR := ∅ |}.
+          set I1' := <[c := Ic1']> (<[p := Ip1']> I1).
+          set s1' := (FP1, C1, Mk1, Nx1', Ky1, I1'): snapshot.
+          set M1' := <[T1 + 1 := s1']> M1.
+          
+
+
+        * iDestruct "SShot1" as %[FP1 [C1 [Mk1 [Nx1 [Ky1 [I1 
+            [Hs1 [Dom_Mk1 [Dom_Nx1 [Dom_Ky1 Dom_I1]]]]]]]]]].
+          set Nx1' := <[p := next']> Nx1.
+          set s1' := (FP1, C1, Mk1, Nx1', Ky1, I1): snapshot.
+          set M1' := <[T1 + 1 := s1']> M1.
+          iAssert (⌜per_tick_inv s1⌝)%I as %PT_s1.
+          { iDestruct "Hist" as (M')"(_&_&_&%&_)". iPureIntro.
+            apply leibniz_equiv in Habs1. rewrite <-Habs1.
+            by apply PT1. }
+          iAssert (hist γ_t γ_m M1' (T1+1))%I with "[Hist]" as "Hist".
+          { admit. }
+          iAssert (▷ helping_inv N γ_t γ_r γ_td1 γ_td2 γ_ght M1')%I with
+            "[Help]" as "Help".
+          { admit. }
+          iAssert (past_state γ_m t0 s1')%I as "Past_s1'".
+          { admit. }
+          assert (FP s1' = FP s1) as FP_s1'.
+          { by rewrite /FP /s1' Hs1. }
+          assert (abs s1' = abs s1) as Habs'.
+          { by rewrite /abs /s1' Hs1. }
+          iAssert (dsRepI γ_r (abs s1'))%I with "[Ds]" as "Ds".
+          { by rewrite Habs'. }
+          iAssert (own γ_ks (● prodKS (KS, abs s1')))%I with "[GKS]" as "GKS".
+          { by rewrite Habs'. }
+          assert (∀ n, n ≠ p → Next s1' n = Next s1 n) as HN.
+          { intros n Hnc. 
+            rewrite /Next /s1' Hs1 /= /Nx1' lookup_insert_ne; try done. }
+          assert (Next s1' p = <[i:=cn]> (Next s1 p)) as HNp.
+          { by rewrite /s1' Hs1 /Next /Nx1' lookup_insert Def_next' /Next Hs1. }
+          assert (∀ n, Key s1' n = Key s1 n) as HK.
+          { by rewrite /Key /s1' Hs1 /=. }
+          assert (∀ n, FI s1' n = FI s1 n) as HI.
+          { by rewrite /FI /s1' Hs1 /=. }
+          assert (∀ n, Mark s1' n = Mark s1 n) as HM.
+          { by rewrite /FI /s1' Hs1. }
+          assert (p ≠ tl) as p_neq_tl. admit.
+          assert (Key s1 p < Key s1 cn) as Key_pcn. admit.
+          assert (cn ∈ FP s1) as FP_cn1. admit.
+          iAssert (⌜snapshot_constraints s1'⌝)%I as "SShot1'".
+          { iPureIntro. exists FP1, C1, Mk1, Nx1', Ky1, I1.
+            repeat split; try done.
+            rewrite /Nx1'. rewrite dom_insert_L.
+            assert (p ∈ dom Nx1). 
+            { rewrite Hs1 in FP_p1. rewrite Dom_Nx1. by unfold FP in FP_p1. }
+            clear -H Dom_Nx1. set_solver. }
+          assert (per_tick_inv s1') as PT_s1'.
+          { destruct PT_s1 as (PT1'&PT2'&PT3'&PT4'&PT5').
+            split; last split; last split; last split.
+            - destruct PT1' as (PT11'&PT12'&PT13'&PT14'&PT15'). repeat split.
+              + intros i'. rewrite /Marki HM. apply PT11'.
+              + rewrite HK. apply PT12'.
+              + rewrite HK. apply PT13'.
+              + by rewrite FP_s1'.
+              + by rewrite FP_s1'.
+            - rewrite /s1' /GFI /FP /FI. by rewrite Hs1 /GFI /FP /FI in PT2'.
+            - intros n Hn. rewrite FP_s1' in Hn. apply PT3' in Hn.
+              destruct (decide (n = p)) as [-> | Hnp].
+              + rewrite HNp HK HI HM.
+                destruct Hn as (Hn1&Hn2&Hn3&Hn4&Hn5&Hn6).
+                split; last split; last split; last split; last split; try done.
+                * intros i'. destruct (decide (i' = i)) as [-> | Hi'i].
+                  rewrite lookup_insert. split; try done.
+                  rewrite lookup_insert_ne; try done.
+                * rewrite dom_insert. clear -Hn3; set_solver.
+                * rewrite lookup_insert_ne; try done.
+              + rewrite HK HI HM. rewrite HN; try done.
+            - intros n1 n2 i'. destruct (decide (n1 = p)) as [-> | Hn1p].
+              + rewrite /Nexti HNp !HK. destruct (decide (i = i')) as [-> | Hi'i].
+                rewrite lookup_insert. intros [=<-]. done. 
+                rewrite lookup_insert_ne; try done. apply PT4'.
+              + rewrite !HK /Nexti HN; try done. apply PT4'. 
+            - intros n1 n2 i'. rewrite FP_s1'. 
+              destruct (decide (n1 = p)) as [-> | Hn1p].
+              + rewrite /Nexti HNp. destruct (decide (i = i')) as [-> | Hi'i].
+                rewrite lookup_insert. intros [=<-]. done. 
+                rewrite lookup_insert_ne; try done. apply PT5'.
+              + rewrite /Nexti HN; try done. apply PT5'. }
+          assert (transition_inv s1 s1') as Trans_s1.
+          { repeat split; try rewrite FP_s1'; try done; last first.
+            - intros n i' Hfp. rewrite /Marki HM. done.
+            - intros n. rewrite /Marki HM. intros H' H''. 
+              rewrite H' in H''; try done. }
+          iAssert (resources γ_ks s1')%I 
+            with "[GKS Nodes_KS Node_p Nodes_rest]" as "Res".
+          { iFrame "GKS". rewrite FP_s1'. iSplitR "Nodes_KS".
+            rewrite (big_opS_delete _ (FP s1) p); try done.
+            iSplitL "Node_p". rewrite Def_next' HNp HM HK. done.
+            iApply (big_sepS_mono with "Nodes_rest"); try done.
+            intros x Hx. iIntros "Hn". rewrite HK HM HN. done.
+            clear -Hx; set_solver.
+            iApply (big_sepS_mono with "Nodes_KS"); try done.
+            intros x Hx. iIntros "Hn". rewrite HI.
+            assert (Content s1' x = Content s1 x) as ->.
+            rewrite /Content HK /Marki HM. done. done. }
+
+          iAssert (∃ s, past_state γ_m t0 s ∗ ⌜traversal_inv s i k p cn⌝)%I 
+            as "#HtrInv'".
+          { iExists s1'. iFrame "#". iPureIntro. repeat split.
+            rewrite FP_s1'; try done. rewrite FP_s1'; try done.
+            admit. rewrite /Marki HM Mark_p1. done. rewrite /Nexti HNp.
+            by rewrite lookup_insert. }  
+          iModIntro. iSplitR "Hpost".
+          { iNext. iExists M1', (T1+1), s1'. iFrame "∗#%".
+            iPureIntro; rewrite /M1'; split; last split.
+            - by rewrite lookup_total_insert.
+            - intros t Ht. destruct (decide (t = T1+1)) as [-> | Ht'].
+              + by rewrite lookup_total_insert.
+              + rewrite lookup_total_insert_ne; try done. apply PT1.
+                rewrite dom_insert in Ht. clear -Ht' Ht; set_solver.
+            - intros t Ht. destruct (decide (t = T1)) as [-> | Ht'].
+              + rewrite lookup_total_insert. rewrite lookup_total_insert_ne.
+                apply leibniz_equiv in Habs1. by rewrite Habs1. clear; lia.
+              + rewrite !lookup_total_insert_ne. apply Trans_M1.
+                all: clear -Ht Ht'; lia. }
+          wp_pures.
+          iApply "IH"; try done.
+      + iDestruct "Hsuccess" as %[Hcond ->].
         iModIntro. iSplitR "Hpost".
-        { iNext. iExists M1, T1, s1.
-          iFrame "∗%".
+        { iNext. iExists M1, T1, s1. iFrame "∗%".
           rewrite (big_sepS_delete _ (FP s1) p); last by eauto.
-          iFrame "Res_rest". admit. }
-        wp_pures.
-        iApply "IH"; try done.
-      + iDestruct "Hif" as "%H'". 
-        destruct H' as [Mark_p1 ->].
-        iModIntro. iSplitR "Hpost".
-        { iNext. iExists M1, T1, s1.
-          iFrame "∗%".
-          rewrite (big_sepS_delete _ (FP s1) p); last by eauto.
-          iFrame "Res_rest". iFrame. }
-        wp_pures.
-        (* Restart case *) admit.  
+          iFrame "Nodes_rest". iFrame. }
+        wp_pures. iSpecialize ("Hpost" $! None). by iApply "Hpost".
     - awp_apply compareKey_spec. 
       iInv "HInv" as (M1 T1 s1) "(>Ds & >%Habs1 & >Hist & Help & >Templ)".
       { admit. }
-      iDestruct "Templ" as "(Hglob & Res & %PT1 & %Trans_M1)". 
-      set γ_I := skiplist_v1.SKIPLIST1.γ_I.
-      set γ_fp := skiplist_v1.SKIPLIST1.γ_fp.
-      set γ_ks := skiplist_v1.SKIPLIST1.γ_ks.
+      iDestruct "Templ" as "(SShot1 & Res & %PT1 & %Trans_M1)".
+      iDestruct "Res" as "(GKS & Nodes & Nodes_KS)".
       iAssert (⌜c ∈ FP s1⌝)%I as %FP_c1.
       { (* interpolation *) admit. }
       rewrite (big_sepS_delete _ (FP s1) c); last by eauto.
-      iDestruct "Res" as "((Node_c & Node_crest) & Res_rest)".
+      iDestruct "Nodes" as "(Node_c & Nodes_rest)".
       iAaccIntro with "Node_c".
-      { iIntros "Node". iModIntro. iFrame.
-        iNext; iExists M1, T1, s1.
-        iFrame "∗%#". 
-        rewrite (big_sepS_delete _ (FP s1) c); last by eauto. 
-        iFrame "Res_rest". iFrame. }
-      iIntros (res)"(Node_c & Hif)".
+      { iIntros "Node_c". iModIntro. iFrame "Hpost".
+        iNext; iExists M1, T1, s1. iFrame "∗%#". 
+        rewrite (big_sepS_delete _ (FP s1) c); last by eauto. iFrame. }
+      iIntros (res)"(Node_c & %Hif)".
       iAssert (past_state γ_m t0 s1) as "#Hs1".
       { admit. }
-      iModIntro. iSplitR "Hpost Hif".
-      { iNext. iExists M1, T1, s1.
-        iFrame "∗%".
+      iModIntro. iSplitR "Hpost".
+      { iNext. iExists M1, T1, s1. iFrame "∗%".
         rewrite (big_sepS_delete _ (FP s1) c); last by eauto.
-        iFrame "Res_rest". iFrame. }
+        iFrame "Nodes_rest". iFrame. }
       wp_pures.
-      destruct (decide_rel eq #res #0); first last.
-      + wp_pures. destruct (decide_rel eq #res #1); first last.
-        * wp_pures. iModIntro; by iApply "Hpost". 
-        * destruct (decide (res = 0)).
-          { subst res. exfalso; apply n. apply f_equal.
-            eauto. }
-          destruct (decide (res = 1)); wp_pures; iModIntro; by iApply "Hpost". 
-      + wp_pures. 
-        destruct (decide (res = 0)); last first.
-        { clear -e n. exfalso. injection e. intros H'.
-          apply n. lia. }
-        iDestruct "Hif" as %Key_c1.  
-        iApply "IH"; try done.
-        iExists s0. admit.
+      destruct (bool_decide (#res = #0)) eqn: Hbool; first last.
+      + rewrite bool_decide_eq_false in Hbool.
+        assert (res ≠ 0) as Hres0. { intros ->. by apply Hbool. } 
+        wp_pures. destruct (bool_decide (#res = #1)) eqn:Hbool1; first last.
+        * wp_pures. iModIntro. iSpecialize ("Hpost" $! (Some (p,c,false))).
+          iEval (rewrite /=) in "Hpost". iApply "Hpost".
+          iDestruct "HtrInv" as (s)"(Past_s & Hpc)".
+          iExists s. iFrame "#". admit.  
+        * rewrite bool_decide_eq_true in Hbool1. inversion Hbool1.
+          assert (res = 1) as -> by lia.
+          wp_pures. iModIntro. iSpecialize ("Hpost" $! (Some (p,c,true))).
+          iEval (rewrite /=) in "Hpost". iApply "Hpost".
+          iDestruct "HtrInv" as (s)"(Past_s & Hpc)".
+          iExists s. iFrame "#". admit.  
+      + wp_pures. iApply "IH". { iExists s0. admit. }
+        iFrame.
     - (* Contradiction case *) admit.
-    - iModIntro; by iApply "Hpost".
+    - iModIntro. iSpecialize ("Hpost" $! (Some (p,c,false))). 
+      iEval (rewrite /=) in "Hpost". iApply "Hpost".
+      iDestruct "HtrInv" as (s)"(Past_s & Hpc)".
+      iExists s. iFrame "#". admit.  
   Admitted.
 
-  Lemma traverse_pop_spec N γ_t γ_s γ_m γ_td γ_ght γ_sy t_id t0 k 
-                           (i: nat) preds succs ps ss:
-      main_inv N γ_t γ_s γ_m γ_td γ_ght -∗
-        thread_vars γ_t γ_ght γ_sy t_id t0 -∗  
-        {{{  is_array preds ps ∗ is_array succs ss 
-              ∗ (∀ j, ⌜i < j < L⌝ → 
-                  ∃ s, past_state γ_m t0 s 
-                      ∗ ⌜traversal_inv s j k (ps !!! j) (ss !!! j)⌝)  }}}
-           traverse_pop #k #preds #succs #i%nat
-        {{{ (ps' ss': list Node) (res: bool), 
-              RET (#preds, #succs, #res);
-              is_array preds ps' ∗ is_array succs ss' 
-              ∗ (∀ j, ⌜i - 1 < j < L⌝ → 
+  Lemma traverse_pop_spec N γ_t γ_r γ_m γ_td1 γ_td2 γ_ght
+    γ_sy t_id t0 k preds succs ps0 ss0 (i: nat):
+    main_inv N γ_t γ_r γ_m γ_td1 γ_td2 γ_ght -∗
+      thread_vars γ_t γ_ght γ_sy t_id t0 -∗  
+        {{{ is_array preds ps0 ∗ is_array succs ss0
+            ∗ (∀ j, ⌜i < j < L⌝ → 
                       ∃ s, past_state γ_m t0 s 
-                          ∗ ⌜traversal_inv s j k (ps' !!! j) (ss' !!! j)⌝) }}}.
+                          ∗ ⌜traversal_inv s j k (ps0 !!! j) (ss0 !!! j)⌝) }}}
+          traverse_pop traverse_rec #k #preds #succs #i
+        {{{ (ores: option (loc * loc * bool)) (ps ss: list Node) (b: bool), 
+              RET (match ores with 
+                    None => NONEV 
+                  | Some res => SOMEV (#res.1.1,#res.1.2,#res.2) end);
+              match ores with 
+                None => is_array preds ps0 ∗ is_array succs ss0
+              | Some res =>
+                ⌜res.1.1 = preds⌝ ∗ ⌜res.1.2 = succs⌝ ∗ ⌜res.2 = b⌝
+              ∗ is_array preds ps ∗ is_array succs ss
+              ∗ (∀ j, ⌜i-1 < j < L⌝ → 
+                      ∃ s, past_state γ_m t0 s 
+                          ∗ ⌜traversal_inv s j k (ps !!! j) (ss !!! j)⌝)
+              ∗ (⌜i = 0⌝ →  let p := ps !!! 0 in
+                            let c := ss !!! 0 in
+                            (∃ s, past_state γ_m t0 s 
+                            ∗ ⌜traversal_inv s 0 k p c⌝
+                            ∗ ⌜if b then k ∈ keyset (FI s c) ∧ k = Key s c
+                                else k ∉ abs s⌝)) end }}}.
   Proof.
     iIntros "#HInv #Thd". iIntros (Φ) "!# Hpre Hpost".
-    iDestruct "Hpre" as "(Hpreds & Hsuccs & #HtrInv)".
-    wp_lam. wp_pures.
-    wp_bind (! _)%E.
+    iDestruct "Hpre" as "(Hpreds & Hsuccs & Hj)". wp_lam. wp_pures.
     iEval (rewrite /is_array) in "Hpreds".
-    assert (is_Some (ps !! (i+1))) as Hpred.
-    { admit. }
-    destruct Hpred as [p Hpred].
+    assert (is_Some (ps0 !! (i+1))) as [p Hp].
+    { admit. } 
     assert (Z.of_nat (i+1) = (Z.of_nat i + 1)%Z) as H' by lia.
     iEval (rewrite <-H').
-    wp_apply (wp_load_offset _ _ _ (DfracOwn 1) (i+1) ((λ n : nat, #n) <$> ps) #p
+    wp_apply (wp_load_offset _ _ _ (DfracOwn 1) (i+1) ((λ n : loc, #n) <$> ps0) #p
       with "[Hpreds]"); try done.
     { admit. }
     { iNext. admit. }
     iIntros "Hpreds".
-    iAssert (is_array preds ps) with "[Hpreds]" as "Hpreds".
+    iAssert (is_array preds ps0) with "[Hpreds]" as "Hpreds".
     { unfold is_array. admit. }
     wp_pures. wp_bind (findNext _ _)%E. 
     awp_apply findNext_spec.
     iInv "HInv" as (M0 T0 s0) "(>Ds & >%Habs0 & >Hist & Help & >Templ)".
     { admit. }
-    iDestruct "Templ" as "(Hglob & Res & %PT0 & %Trans_M0)". 
-    set γ_I := skiplist_v1.SKIPLIST1.γ_I.
-    set γ_fp := skiplist_v1.SKIPLIST1.γ_fp.
-    set γ_ks := skiplist_v1.SKIPLIST1.γ_ks.
+    iDestruct "Templ" as "(SShot0 & Res & %PT0 & %Trans_M0)".
+    iDestruct "Res" as "(GKS & Nodes & Nodes_KS)".
     iAssert (⌜p ∈ FP s0⌝)%I as %FP_p0.
     { (* interpolation *) admit. }
     rewrite (big_sepS_delete _ (FP s0) p); last by eauto.
-    iDestruct "Res" as "((Node_p & Node_prest) & Res_rest)".
+    iDestruct "Nodes" as "(Node_p & Nodes_rest)".
     iAaccIntro with "Node_p".
-    { iIntros "Node". iModIntro. iFrame.
-      iNext; iExists M0, T0, s0.
-      iFrame "∗%#". 
-      rewrite (big_sepS_delete _ (FP s0) p); last by eauto. 
-      iFrame "Res_rest". iFrame. }
+    { iIntros "Node_p". iModIntro. iFrame "Hpost Hpreds Hsuccs Hj".
+      iNext; iExists M0, T0, s0. iFrame "∗%#". 
+      rewrite (big_sepS_delete _ (FP s0) p); last by eauto. iFrame. }
     iIntros (m c) "(Node_p & %Mark_p0 & %Next_p0)".
-    iModIntro. iSplitR "Hpreds Hsuccs Hpost".
-    { iNext. iExists M0, T0, s0.
-      iFrame "∗%".
-      rewrite (big_sepS_delete _ (FP s0) p); last by eauto.
-      iFrame "Res_rest". iFrame. }
-    clear γ_I γ_fp γ_ks.
+    iModIntro. iSplitR "Hpreds Hsuccs Hpost Hj".
+    { iNext. iExists M0, T0, s0. iFrame "∗%".
+      rewrite (big_sepS_delete _ (FP s0) p); last by eauto. iFrame. }
     destruct c as [c |]; last first; wp_pures.
-    + (* Contradiction case *) admit.
-    + wp_apply traverse_i_spec_high; try done.
-      { admit. }
-      iIntros (p' c' res)"#HtrInv_p'".
-      wp_pures. wp_bind (_ <- _)%E. 
-      iApply (array_store with "[Hpreds]").
-      { iFrame "Hpreds". iPureIntro. admit. }
-      iNext. iIntros "Hpreds". 
-      wp_pures. wp_bind (_ <- _)%E. 
-      iApply (array_store with "[Hsuccs]").
-      { iFrame "Hsuccs". iPureIntro. admit. }
-      iNext. iIntros "Hsuccs". wp_pures.
-      iApply ("Hpost"). iModIntro; iFrame.
-      iIntros (j)"%Hj". destruct (decide (j = i)) as [-> | Hij].
-      - assert (<[i:=p']> ps !!! i = p') as H1'. 
-        (* rewrite lookup_total_insert. *)
-        admit.
-        assert (<[i:=c']> ss !!! i = c') as H1''. 
-        admit. 
-        by rewrite H1' H1''.
-      - assert (<[i := p']> ps !!! j = ps !!! j) as H1'. 
-        admit. 
-        assert (<[i := c']> ss !!! j = ss !!! j) as H1''. 
-        admit. 
-        rewrite H1' H1''. iApply "HtrInv". 
-        iPureIntro; lia.
+    { (* Contradiction case *) admit. }
+    iAssert (∃ s : snapshot, past_state γ_m t0 s ∗ ⌜traversal_inv s i k p c⌝)%I
+      as "Hpc". { admit. }
+    wp_apply traverse_i_spec; try done.
+    iIntros (ores) "Hores".
+    destruct ores as [[[p' c'] b]|]; last first.
+    { wp_pures. iSpecialize ("Hpost" $! None ps0 ss0 true). iApply "Hpost".
+      iFrame. done. }
+    wp_pures. wp_bind (_ <- _)%E. 
+    iApply (array_store with "[Hpreds]").
+    { iFrame "Hpreds". admit. }
+    iIntros "!> Hpreds". wp_pures. wp_bind (_ <- _)%E. 
+    iApply (array_store with "[Hsuccs]").
+    { iFrame "Hsuccs". admit. }
+    iIntros "!> Hsuccs". wp_pures.
+    iSpecialize ("Hpost" $! (Some (preds,succs,b)) _ _ b).
+    iEval (rewrite /=) in "Hpost Hores". iApply "Hpost".
+    iModIntro. iFrame "∗%". repeat (iSplitR; first by iPureIntro).
+    iDestruct "Hores" as (s)"(Past_s & Hpc' & %Hi0)".
+    iSplit. iIntros (j)"%Hj". destruct (decide (j = i)) as [-> | Hij].
+    { iExists s. rewrite !list_lookup_total_insert. iFrame. all: admit. }
+    iAssert (⌜i < j < L⌝)%I as "Hj'". { iPureIntro. lia. }
+    iPoseProof ("Hj" with "Hj'") as (s')"(Past_s' & Htr)".
+    iExists s'. rewrite !list_lookup_total_insert_ne; try done. iFrame.
+    iIntros "%". subst i. rewrite !list_lookup_total_insert.
+    iExists s. iFrame. iPureIntro. by apply Hi0. all: admit.
   Admitted.
 
 
-  Lemma traverse_loop_rec_spec N γ_t γ_s γ_m γ_td γ_ght γ_sy t_id t0 k 
-                           (i: nat) preds succs ps ss:
-      main_inv N γ_t γ_s γ_m γ_td γ_ght -∗
-        thread_vars γ_t γ_ght γ_sy t_id t0 -∗  
-        {{{  is_array preds ps ∗ is_array succs ss 
-              ∗ (∀ j, ⌜i < j < L⌝ → 
+  Lemma traverse_rec_spec N γ_t γ_r γ_m γ_td1 γ_td2 γ_ght γ_sy t_id 
+    t0 k preds succs ps0 ss0 (i: nat):
+    main_inv N γ_t γ_r γ_m γ_td1 γ_td2 γ_ght -∗
+      thread_vars γ_t γ_ght γ_sy t_id t0 -∗  
+      {{{ is_array preds ps0 ∗ is_array succs ss0
+          ∗ (∀ j, ⌜i < j < L⌝ → 
                   ∃ s, past_state γ_m t0 s 
-                      ∗ ⌜traversal_inv s j k (ps !!! j) (ss !!! j)⌝)  }}}
-           traverse_loop_rec #k #preds #succs #i%nat
-        {{{ (ps' ss': list Node), 
-              RET #();
-              is_array preds ps' ∗ is_array succs ss' 
-              ∗ (∀ i, ⌜1 ≤ i < L⌝ → 
-                      ∃ s, past_state γ_m t0 s 
-                          ∗ ⌜traversal_inv s i k (ps' !!! i) (ss' !!! i)⌝) }}}.
+                  ∗ ⌜traversal_inv s j k (ps0 !!! j) (ss0 !!! j)⌝) }}}
+        traverse_rec #k #preds #succs #i
+      {{{ (ps ss: list Node) (res: bool), 
+            RET (#preds, #succs, #res);
+            is_array preds ps ∗ is_array succs ss
+          ∗ (∀ i, ⌜i < L⌝ → ∃ s, past_state γ_m t0 s 
+                          ∗ ⌜traversal_inv s i k (ps !!! i) (ss !!! i)⌝
+                          ∗ ⌜i = 0 → let c := ss !!! 0 in
+                                      if res then 
+                                        k ∈ keyset (FI s c) ∧ k = Key s c
+                                      else 
+                                        k ∉ abs s⌝ ) }}}.
   Proof.
-    iIntros "#HInv #Thd". iIntros (Φ) "!# Hpre Hpost".
-    iLöb as "IH" forall (i ps ss). 
-    iDestruct "Hpre" as "(Hpreds & Hsuccs & #HtrInv)".
-    wp_lam. wp_pures.
-    destruct (decide_rel Z.le 1%nat i); first last.
-    - iEval (unfold bool_decide); wp_pures.
-      assert (i < 1) by lia.
-      iApply "Hpost". iModIntro.
-      iFrame "Hpreds Hsuccs".
-      iIntros (i') "%Hi". iApply "HtrInv".
-      iPureIntro; lia.
-    - iEval (unfold bool_decide); wp_pures.
-      wp_apply (traverse_pop_spec with "[] [] [Hpreds Hsuccs]"); try done.
-      { iFrame "Hpreds Hsuccs". try done. }
-      iIntros (ps' ss' res) "(Hpreds & Hsuccs & #HtrInv')". wp_pures.
-      iSpecialize ("IH" $! (i-1) ps' ss').
-      assert (Z.of_nat (i-1) = (Z.of_nat i - 1)%Z) as H' by lia.
-      iEval (rewrite H') in "IH".
-      iApply ("IH" with "[$Hpreds $Hsuccs]"); try done.
-  Admitted.
-
-
-  Lemma traverse_loop_spec N γ_t γ_s γ_m γ_td γ_ght γ_sy t_id t0 k 
-                           preds succs ps ss:
-      main_inv N γ_t γ_s γ_m γ_td γ_ght -∗
-        thread_vars γ_t γ_ght γ_sy t_id t0 -∗  
-        {{{ is_array preds ps ∗ is_array succs ss 
-            ∗ (∃ s, past_state γ_m t0 s 
-                    ∗ ⌜traversal_inv s (L-1) k (ps !!! (L-1)) (ss !!! (L-1))⌝) }}}
-           traverse_loop #k #preds #succs
-        {{{ (ps' ss': list Node), 
-              RET #();
-              is_array preds ps' ∗ is_array succs ss' 
-              ∗ (∀ i, ⌜1 ≤ i < L⌝ → 
-                  ∃ s, past_state γ_m t0 s 
-                        ∗ ⌜traversal_inv s i k (ps' !!! i) (ss' !!! i)⌝) }}}.
-  Proof.
-    iIntros "#HInv #Thd". iIntros (Φ) "!# Hpre Hpost".
-    iDestruct "Hpre" as "(Hpreds & Hsuccs & #HtrInv)".
-    wp_lam. wp_pures.
-    assert (L > 1). admit.
-    wp_apply (traverse_loop_rec_spec with "[] [] [Hpreds Hsuccs]"); try done.
-    iFrame "Hpreds Hsuccs".
-    iIntros (j) "%Hj".
-    assert (j = L-1) as -> by lia.
-    try done.
-  Admitted.
-
-
-  Lemma traverse_i_spec_base N γ_t γ_s γ_m γ_td γ_ght γ_sy t_id t0 k 
-                           (i: nat) (p c: Node):
-      main_inv N γ_t γ_s γ_m γ_td γ_ght -∗
-        thread_vars γ_t γ_ght γ_sy t_id t0 -∗  
-        {{{ ∃ s, past_state γ_m t0 s ∗ ⌜k ∈ insets (FI s p)⌝
-                  ∗ ⌜Marki s p 0 = false⌝ ∗ ⌜k ∈ outset _ (FI s p) c⌝ }}}
-           traverse_i #0%nat #k #p #c
-        {{{ (p' c': Node) (res: bool), 
-              RET (#p', #c', #res);
-              if res then 
-                ∃ s, past_state γ_m t0 s 
-                ∗ ⌜k ∈ keyset (FI s c')⌝
-                ∗ ⌜k = Key s c'⌝
-              else
-                ∃ s, past_state γ_m t0 s 
-                ∗ ⌜k ∉ abs s⌝ }}}.
-  Proof.
-    iIntros "#HInv #Thd". iLöb as "IH" forall (p c).
-    iIntros (Φ) "!# #HtrInv Hpost". wp_lam. wp_pures.
-    awp_apply findNext_spec.
-    iInv "HInv" as (M0 T0 s0) "(>Ds & >%Habs0 & >Hist & Help & >Templ)".
-    { admit. }
-    iDestruct "Templ" as "(Hglob & Res & %PT0 & %Trans_M0)". 
-    set γ_I := skiplist_v1.SKIPLIST1.γ_I.
-    set γ_fp := skiplist_v1.SKIPLIST1.γ_fp.
-    set γ_ks := skiplist_v1.SKIPLIST1.γ_ks.
-    iAssert (⌜c ∈ FP s0⌝)%I as %FP_c0.
-    { (* interpolation *) admit. }
-    rewrite (big_sepS_delete _ (FP s0) c); last by eauto.
-    iDestruct "Res" as "((Node_c & Node_crest) & Res_rest)".
-    iAaccIntro with "Node_c".
-    { iIntros "Node". iModIntro. iFrame.
-      iNext; iExists M0, T0, s0.
-      iFrame "∗%#". 
-      rewrite (big_sepS_delete _ (FP s0) c); last by eauto. 
-      iFrame "Res_rest". iFrame. }
-    iIntros (m c') "(Node_c & %Mark_c0 & %Next_c0)".
-    iModIntro. iSplitR "Hpost".
-    { iNext. iExists M0, T0, s0.
-      iFrame "∗%".
-      rewrite (big_sepS_delete _ (FP s0) c); last by eauto.
-      iFrame "Res_rest". iFrame. }
-    clear γ_I γ_fp γ_ks.
-    destruct c' as [c' |]; destruct m; wp_pures. 
-    - awp_apply try_constraint_traverse_spec; try done.
-      iInv "HInv" as (M1 T1 s1) "(>Ds & >%Habs1 & >Hist & Help & >Templ)".
-      { admit. }
-      iDestruct "Templ" as "(Hglob & Res & %PT1 & %Trans_M1)". 
-      set γ_I := skiplist_v1.SKIPLIST1.γ_I.
-      set γ_fp := skiplist_v1.SKIPLIST1.γ_fp.
-      set γ_ks := skiplist_v1.SKIPLIST1.γ_ks.
-      iAssert (⌜p ∈ FP s1⌝)%I as %FP_p1.
-      { (* interpolation *) admit. }
-      iAssert (past_state γ_m t0 s1) as "#Hs1".
-      { admit. }
-      rewrite (big_sepS_delete _ (FP s1) p); last by eauto.
-      iDestruct "Res" as "((Node_p & Node_prest) & Res_rest)".
-      iAaccIntro with "Node_p".
-      { iIntros "Node". iModIntro. iFrame.
-        iNext; iExists M1, T1, s1.
-        iFrame "∗%#". 
-        rewrite (big_sepS_delete _ (FP s1) p); last by eauto. 
-        iFrame "Res_rest". iFrame. }
-      iIntros (success next')"(Node_p & Hif)".
-      destruct success.
-      + iDestruct "Hif" as "%H'".
-        destruct H' as [Mark_p1 [Next_p1 Def_next']].
-        iAssert (∃ s, past_state γ_m t0 s ∗ ⌜traversal_inv s i k p c'⌝)%I 
-          as "#HtrInv'".
-        { iExists s1. iFrame "Hs1". iPureIntro.
-          split; try done. admit. admit. }  
-        iModIntro. iSplitR "Hpost".
-        { iNext. iExists M1, T1, s1.
-          iFrame "∗%".
-          rewrite (big_sepS_delete _ (FP s1) p); last by eauto.
-          iFrame "Res_rest". admit. }
-        wp_pures.
-        iApply "IH"; try done.
-        admit.
-      + iDestruct "Hif" as "%H'". 
-        destruct H' as [Mark_p1 ->].
-        iModIntro. iSplitR "Hpost".
-        { iNext. iExists M1, T1, s1.
-          iFrame "∗%".
-          rewrite (big_sepS_delete _ (FP s1) p); last by eauto.
-          iFrame "Res_rest". iFrame. }
-        wp_pures.
-        (* Restart case *) admit.  
-    - awp_apply compareKey_spec. 
-      iInv "HInv" as (M1 T1 s1) "(>Ds & >%Habs1 & >Hist & Help & >Templ)".
-      { admit. }
-      iDestruct "Templ" as "(Hglob & Res & %PT1 & %Trans_M1)". 
-      set γ_I := skiplist_v1.SKIPLIST1.γ_I.
-      set γ_fp := skiplist_v1.SKIPLIST1.γ_fp.
-      set γ_ks := skiplist_v1.SKIPLIST1.γ_ks.
-      iAssert (⌜c ∈ FP s1⌝)%I as %FP_c1.
-      { (* interpolation *) admit. }
-      rewrite (big_sepS_delete _ (FP s1) c); last by eauto.
-      iDestruct "Res" as "((Node_c & Node_crest) & Res_rest)".
-      iAaccIntro with "Node_c".
-      { iIntros "Node". iModIntro. iFrame.
-        iNext; iExists M1, T1, s1.
-        iFrame "∗%#". 
-        rewrite (big_sepS_delete _ (FP s1) c); last by eauto. 
-        iFrame "Res_rest". iFrame. }
-      iIntros (res)"(Node_c & Hif)".
-      iAssert (past_state γ_m t0 s1) as "#Hs1".
-      { admit. }
-      iModIntro. iSplitR "Hpost Hif".
-      { iNext. iExists M1, T1, s1.
-        iFrame "∗%".
-        rewrite (big_sepS_delete _ (FP s1) c); last by eauto.
-        iFrame "Res_rest". iFrame. }
-      wp_pures.
-      (*
-      destruct (decide_rel eq #res #0); first last.
-      + wp_pures. destruct (decide_rel eq #res #1); first last.
-        * wp_pures. iModIntro; by iApply "Hpost". 
-        * destruct (decide (res = 0)).
-          { subst res. exfalso; apply n. apply f_equal.
-            eauto. }
-          destruct (decide (res = 1)); wp_pures; iModIntro; by iApply "Hpost". 
-      + wp_pures. 
-        destruct (decide (res = 0)); last first.
-        { clear -e n. exfalso. injection e. intros H'.
-          apply n. lia. }
-        iDestruct "Hif" as %Key_c1.  
-        iApply "IH"; try done.
-        iExists s0. admit.
-    - (* Contradiction case *) admit.
-    - iModIntro; by iApply "Hpost".
-    *)
-  Admitted.
-
-  Lemma traverse_pop_spec_base N γ_t γ_s γ_m γ_td γ_ght γ_sy t_id t0 k 
-                           preds succs ps ss:
-      main_inv N γ_t γ_s γ_m γ_td γ_ght -∗
-        thread_vars γ_t γ_ght γ_sy t_id t0 -∗  
-        {{{  is_array preds ps ∗ is_array succs ss 
-             ∗ (∀ i, ⌜1 ≤ i < L⌝ → 
-                  ∃ s, past_state γ_m t0 s 
-                        ∗ ⌜traversal_inv s i k (ps !!! i) (ss !!! i)⌝)  }}}
-           traverse_pop #k #preds #succs #0%nat
-        {{{ (preds succs: loc) (ps' ss': list Node) (p c: Node) (res: bool), 
-              RET (#preds, #succs, #res);
-              is_array preds ps' ∗ is_array succs ss'
-            ∗ (∀ i, ⌜1 ≤ i < L⌝ → 
-                      ∃ s, past_state γ_m t0 s 
-                           ∗ ⌜traversal_inv s i k (ps' !!! i) (ss' !!! i)⌝)
-            ∗ (⌜ps' !!! 0 = p⌝) ∗ (⌜ss' !!! 0 = c⌝)
-            ∗ if res then 
-                ∃ s, past_state γ_m t0 s 
-                ∗ ⌜k ∈ keyset (FI s c)⌝
-                ∗ ⌜k = Key s c⌝
-              else
-                ∃ s, past_state γ_m t0 s 
-                ∗ ⌜k ∉ abs s⌝ }}}.
-  Proof.
-    iIntros "#HInv #Thd". iIntros (Φ) "!# Hpre Hpost".
+    iIntros "#HInv #Thd". iLöb as "IH" forall (i ps0 ss0). 
+    iIntros (Φ) "!# Hpre Hpost".
     iDestruct "Hpre" as "(Hpreds & Hsuccs & #HtrInv)".
     wp_lam. wp_pures. 
-    assert (is_Some (ps !! 1)) as Hpred.
-    { admit. }    
-    destruct Hpred as [p Hpred].
-    assert (Z.of_nat (1) = (Z.of_nat 0 + 1)%Z) as H' by lia.
-    iEval (rewrite <-H').
-    wp_apply (wp_load_offset _ _ _ (DfracOwn 1) (1) ((λ n : nat, #n) <$> ps) #p
-      with "[Hpreds]"); try done.
-    { admit. }
-    { iNext. admit. }
-    iIntros "Hpreds".
-    iAssert (is_array preds ps) with "[Hpreds]" as "Hpreds".
-    { unfold is_array. admit. }
-    wp_pures. wp_bind (findNext _ _)%E. 
-    awp_apply findNext_spec.
-    iInv "HInv" as (M0 T0 s0) "(>Ds & >%Habs0 & >Hist & Help & >Templ)".
-    { admit. }
-    iDestruct "Templ" as "(Hglob & Res & %PT0 & %Trans_M0)". 
-    set γ_I := skiplist_v1.SKIPLIST1.γ_I.
-    set γ_fp := skiplist_v1.SKIPLIST1.γ_fp.
-    set γ_ks := skiplist_v1.SKIPLIST1.γ_ks.
-    iAssert (⌜p ∈ FP s0⌝)%I as %FP_p0.
-    { (* interpolation *) admit. }
-    rewrite (big_sepS_delete _ (FP s0) p); last by eauto.
-    iDestruct "Res" as "((Node_p & Node_prest) & Res_rest)".
-    iAaccIntro with "Node_p".
-    { iIntros "Node". iModIntro. iFrame.
-      iNext; iExists M0, T0, s0.
-      iFrame "∗%#". 
-      rewrite (big_sepS_delete _ (FP s0) p); last by eauto. 
-      iFrame "Res_rest". iFrame. }
-    iIntros (m c) "(Node_p & %Mark_p0 & %Next_p0)".
-    iModIntro. iSplitR "Hpreds Hsuccs Hpost".
-    { iNext. iExists M0, T0, s0.
-      iFrame "∗%".
-      rewrite (big_sepS_delete _ (FP s0) p); last by eauto.
-      iFrame "Res_rest". iFrame. }
-    clear γ_I γ_fp γ_ks.
-    destruct c as [c |]; last first; wp_pures.
-    + (* Contradiction case *) admit.
-    + 
-      (*
-      iApply fupd_wp.
-      iInv "HInv" as (M1 T1 s1) "(>Ds & >%Habs1 & >Hist & Help & >Templ)".
-      iDestruct "Templ" as "(Hglob & Res & %PT1 & %Trans_M1)". 
-      set γ_I := skiplist_v1.SKIPLIST1.γ_I.
-      set γ_fp := skiplist_v1.SKIPLIST1.γ_fp.
-      set γ_ks := skiplist_v1.SKIPLIST1.γ_ks.
-      assert (ps !!! 1 = p) as Hp.
-      { admit. }
-      assert (ps !!! 1 = p) as Hp.
-      { admit. }
-
-
-      iAssert (⌜traversal_inv s i k (ps !!! i) (ss !!! i)⌝)%I as %Htr_pc.
-      iEval (rewrite Hp) in "Hkey".
-      iDestruct "Hkey" as (s)"(Hpast_s & %Key_s_p)".
-      iAssert (⌜k ∈ insets (FI s p)⌝)%I as "%Insets_s_p".
-      { iDestruct "Hpast_s" as (t)"Hpast_s".
-        assert (t ∈ dom M1) as t_in_M1.
-        { admit. }
-        apply PT1 in t_in_M1.
-        assert (M1 !! t = Some s) as M1_t_s.
-        { admit. }
-        unfold lookup_total, map_lookup_total in t_in_M1.
-        rewrite M1_t_s in t_in_M1.
-        simpl in t_in_M1. clear H'.
-        destruct t_in_M1 as [_ [_ [_ H']]].
-        assert (p ∈ FP s) as p_in_s. { admit. }
-        apply H' in p_in_s.
-        destruct p_in_s as [_ [_ [H'' _]]].
-        iPureIntro. apply H''. admit.
-        split; try done. lia. admit. }
-      iModIntro. iSplitR "Hpreds Hsuccs Hpost".
-      { iNext. iExists M1, T1, s1.
-        iFrame "∗%". }
-      clear γ_I γ_fp γ_ks. 
-      iModIntro.
-      *)
-
-      wp_apply traverse_i_spec_base; try done.
-      
-      
-      { admit. }
-      iIntros (p' c' res) "Hres".
-      wp_pures. wp_bind (_ <- _)%E. 
-      iApply (array_store with "[Hpreds]").
-      { iFrame "Hpreds". iPureIntro. admit. }
-      iNext. iIntros "Hpreds". 
-      wp_pures. wp_bind (_ <- _)%E. 
-      iApply (array_store with "[Hsuccs]").
-      { iFrame "Hsuccs". iPureIntro. admit. }
-      iNext. iIntros "Hsuccs". wp_pures.
-      iApply ("Hpost" $! _ _ _ _ p' c'). 
-      iModIntro.
-      iFrame "Hpreds Hsuccs Hres".
-      iSplit. iIntros (i) "%Hi".
-      assert (<[0:=p']> ps !!! i = ps !!! i) as H1'. 
-      admit. rewrite H1'. 
-      assert (<[0:=c']> ss !!! i = ss !!! i) as H1''. 
-      admit. rewrite H1''. 
-      iApply "HtrInv"; try done.
-      iPureIntro; admit.
+    wp_apply (traverse_pop_spec with "[] [] [Hpreds Hsuccs]"); try done.
+    iFrame "∗#". iIntros (ores ps ss b)"Hores".
+    destruct ores as [[[preds' succs'] res] |]; last first.
+    { wp_pures. iDestruct "Hores" as "(Hpreds & Hsuccs)".
+      iApply ("IH" with "[Hpreds Hsuccs]"). iFrame. iIntros (j)"%Hj".
+      assert (j = L-1) as -> by lia. admit. }
+    wp_pures. iDestruct "Hores" as "(%H' & %H'' & %H1' & H1'')". 
+    rewrite /= in H' H'' H1'. subst preds' succs' b.  
+    iDestruct "H1''" as "(Hpreds & Hsuccs & #Hj & Hi0)".
+    destruct (bool_decide (#i = #0)) eqn: Hbool; wp_pures.
+    - rewrite bool_decide_eq_true in Hbool. inversion Hbool. iModIntro.
+      iApply "Hpost". iFrame "Hpreds Hsuccs". 
+      iAssert (⌜i = 0⌝)%I as "Htr0". { iPureIntro; lia. }
+      iDestruct ("Hi0" with "Htr0") as "H'".
+      iIntros (j) "%Hj". destruct (decide (j = 0)) as [-> | Hj0].
+      + iDestruct "H'" as (s)"(Hpast_s & #Htr & Hres)".
+        iExists s; try iFrame "∗#". iIntros "_". iFrame.
+      + iAssert (⌜i - 1 < j < L⌝)%I as "Hj'". { iPureIntro; lia. }
+        iPoseProof ("Hj" with "Hj'") as (s)"(Past_s & Htr)".
+        iExists s. iFrame "#". iIntros "%"; exfalso; lia.
+    - iSpecialize ("IH" $! (i-1) ps ss).
+      rewrite bool_decide_eq_false in Hbool.
+      assert (i ≠ 0). { intros ->. apply Hbool. try done. }
+      assert (Z.sub i 1 = (i-1)%nat) as -> by lia.
+      iApply ("IH" with "[$Hpreds $Hsuccs $Hj]"). done.
   Admitted.
-*)
-    
-  Lemma traverse_spec N γ_t γ_s γ_m γ_td1 γ_td2 γ_ght (h t: Node) γ_sy t_id t0 k:
-      main_inv N γ_t γ_s γ_m γ_td1 γ_td2 γ_ght -∗
-        thread_vars γ_t γ_ght γ_sy t_id t0 -∗  
-        {{{ True }}}
-           traverse #h #t #k
-        {{{ (preds succs: loc) (ps ss: list Node) (p c: Node) (res: bool), 
-              RET (#preds, #succs, #res);
-              is_array preds ps ∗ is_array succs ss
-            ∗ (∀ i, ⌜1 ≤ i < L⌝ → 
-                      ∃ s, past_state γ_m t0 s 
-                           ∗ ⌜traversal_inv s i k (ps !!! i) (ss !!! i)⌝)
-            ∗ (⌜ps !!! 0 = p⌝) ∗ (⌜ss !!! 0 = c⌝)
-            ∗ (∃ s, past_state γ_m t0 s ∗ ⌜p ∈ FP s⌝ ∗ ⌜c ∈ FP s⌝
-                    ∗ if res then ⌜k ∈ keyset (FI s c)⌝ ∗ ⌜k = Key s c⌝
-                      else ⌜k ∉ abs s⌝) }}}.
+
+
+  Lemma traverse_spec N γ_t γ_r γ_m γ_td1 γ_td2 γ_ght γ_sy t_id t0 k:
+    main_inv N γ_t γ_r γ_m γ_td1 γ_td2 γ_ght -∗
+      thread_vars γ_t γ_ght γ_sy t_id t0 -∗  
+      {{{ True }}}
+          traverse #hd #tl #k
+      {{{ (preds succs: loc) (ps ss: list Node) (res: bool), 
+            RET (#preds, #succs, #res);
+            is_array preds ps ∗ is_array succs ss
+          ∗ (∀ i, ⌜i < L⌝ → ∃ s, past_state γ_m t0 s 
+                          ∗ ⌜traversal_inv s i k (ps !!! i) (ss !!! i)⌝
+                          ∗ ⌜i = 0 → let c := ss !!! 0 in
+                                      if res then 
+                                        k ∈ keyset (FI s c) ∧ k = Key s c
+                                      else 
+                                        k ∉ abs s⌝ ) }}}.
   Proof.  
     iIntros "#HInv #Thd". iIntros (Φ) "!# _ Hpost".
-    wp_lam. wp_pures. wp_bind (AllocN _ _)%E. Check array_repeat.
+    wp_lam. wp_pures. wp_bind (AllocN _ _)%E. 
     iApply array_repeat. admit.
     iNext. iIntros (preds) "Hpreds".
     wp_pures. wp_bind (AllocN _ _)%E.
     iApply array_repeat. admit.
-    iNext. iIntros (succs) "Hsuccs".
-    wp_pures. wp_bind (_ <- _)%E. 
-    iApply (array_store with "[Hpreds]").
-    iFrame "Hpreds". { iPureIntro. rewrite replicate_length. admit. }
-    iNext. iIntros "Hpreds".
-    wp_pures. wp_bind (_ <- _)%E. 
-    iApply (array_store with "[Hsuccs]").
-    iFrame "Hsuccs". { iPureIntro. admit. }
-    iNext. iIntros "Hsuccs". wp_pures.
-    wp_apply (traverse_loop_spec with "[] [] [Hpreds Hsuccs]"); try done.
-    { iFrame "Hpreds Hsuccs". admit. }
-    iIntros (ps' ss') "(Hpreds & Hsuccs & #HtrInv)". wp_pures.
-    wp_apply (traverse_pop_spec_base with "[] [] [Hpreds Hsuccs]"); try done.
-    iFrame "Hpreds Hsuccs". iApply "HtrInv".
+    iNext. iIntros (succs) "Hsuccs". wp_pures. 
+    wp_apply (traverse_rec_spec with "[] [] [Hpreds Hsuccs]"); try done.
+    iFrame "Hpreds Hsuccs". iIntros (j) "%Hj". 
+    assert (j = L-1) as -> by lia. rewrite !lookup_total_replicate_2.
+    all : try lia. admit.  
   Admitted.
 
 End SKIPLIST1_SPEC_TRAVERSE.
